Prove lemmas for stsim

src/StateRA.v
@@ -7,6 +7,44 @@ From Fairness Require Import PCM MonotonePCM ThreadsRA ModSim FairBeh.
 
 Set Implicit Arguments.
 
+Section UPD.
+  Variable A: Type.
+  Context `{IN: @GRA.inG (Auth.t (Excl.t A)) Σ}.
+
+  Lemma black_white_update a0 a' a1
+    :
+    (OwnM (Auth.black (Excl.just a0: @Excl.t A)))
+      -∗
+      (OwnM (Auth.white (Excl.just a': @Excl.t A)))
+      -∗
+      #=> (OwnM (Auth.black (Excl.just a1: @Excl.t A)) ** OwnM (Auth.white (Excl.just a1: @Excl.t A))).
+  Proof.
+    iIntros "H0 H1". iCombine "H0 H1" as "H".
+    iPoseProof (OwnM_Upd with "H") as "> [H0 H1]".
+    { apply Auth.auth_update.
+      instantiate (1:=Excl.just a1). instantiate (1:=Excl.just a1).
+      ii. des. ur in FRAME. des_ifs. split.
+      { ur. ss. }
+      { ur. ss. }
+    }
+    iModIntro. iFrame.
+  Qed.
+
+  Lemma black_white_equal a a'
+    :
+    (OwnM (Auth.black (Excl.just a: @Excl.t A)))
+      -∗
+      (OwnM (Auth.white (Excl.just a': @Excl.t A)))
+      -∗
+      ⌜a = a'⌝.
+  Proof.
+    iIntros "H0 H1". iCombine "H0 H1" as "H".
+    iOwnWf "H". ur in H. des.
+    rr in H. des. ur in H. des_ifs.
+  Qed.
+End UPD.
+
+
 Section INVARIANT.
   Variable state_src: Type.
   Variable state_tgt: Type.
@@ -31,7 +69,7 @@ Section INVARIANT.
 
   Definition default_I: TIdSet.t -> (@imap ident_src wf_src) -> (@imap (sum_tid ident_tgt) nat_wf) -> state_src -> state_tgt -> iProp :=
     fun ths im_src im_tgt st_src st_tgt =>
-      (own_threads ths)
+      (own_threads_black ths)
         **
         (OwnM (Auth.black (Excl.just st_src: @Excl.t state_src): stateSrcRA))
         **
@@ -39,8 +77,179 @@ Section INVARIANT.
         **
         (OwnM (Auth.black (Excl.just im_src: @Excl.t (imap ident_src wf_src)): identSrcRA))
         **
-        (OwnM (Auth.black (Excl.just (imap_proj_id2 im_tgt): @Excl.t (imap ident_tgt nat_wf)): identTgtRA))
+        (OwnM (Auth.black (Excl.just (snd (imap_proj_id im_tgt)): @Excl.t (imap ident_tgt nat_wf)): identTgtRA))
         **
-        (OwnM (Auth.black (Excl.just (imap_proj_id1 im_tgt): @Excl.t (imap thread_id nat_wf)): identThsRA))
+        (OwnM (Auth.black (Excl.just (fst (imap_proj_id im_tgt)): @Excl.t (imap thread_id nat_wf)): identThsRA))
   .
+
+  Lemma default_I_update_st_src ths im_src im_tgt st_src0 st_tgt st_src' st_src1
+    :
+    (default_I ths im_src im_tgt st_src0 st_tgt)
+      -∗
+      (OwnM (Auth.white (Excl.just st_src': @Excl.t state_src): stateSrcRA))
+      -∗
+      #=> (OwnM (Auth.white (Excl.just st_src1: @Excl.t state_src)) ** default_I ths im_src im_tgt st_src1 st_tgt).
+  Proof.
+    unfold default_I. iIntros "[[[[[H0 H1] H2] H3] H4] H5] OWN".
+    iPoseProof (black_white_update with "H1 OWN") as "> [H1 OWN]".
+    iModIntro. iFrame.
+  Qed.
+
+  Lemma default_I_update_st_tgt ths im_src im_tgt st_src st_tgt0 st_tgt' st_tgt1
+    :
+    (default_I ths im_src im_tgt st_src st_tgt0)
+      -∗
+      (OwnM (Auth.white (Excl.just st_tgt': @Excl.t state_tgt): stateTgtRA))
+      -∗
+      #=> (OwnM (Auth.white (Excl.just st_tgt1: @Excl.t state_tgt)) ** default_I ths im_src im_tgt st_src st_tgt1).
+  Proof.
+    unfold default_I. iIntros "[[[[[H0 H1] H2] H3] H4] H5] OWN".
+    iPoseProof (black_white_update with "H2 OWN") as "> [H2 OWN]".
+    iModIntro. iFrame.
+  Qed.
+
+  Lemma default_I_update_ident_src ths im_src0 im_tgt st_src st_tgt im_src' im_src1
+    :
+    (default_I ths im_src0 im_tgt st_src st_tgt)
+      -∗
+      (OwnM (Auth.white (Excl.just im_src': @Excl.t (imap ident_src wf_src)): identSrcRA))
+      -∗
+      #=> (OwnM (Auth.white (Excl.just im_src1: @Excl.t (imap ident_src wf_src))) ** default_I ths im_src1 im_tgt st_src st_tgt).
+  Proof.
+    unfold default_I. iIntros "[[[[[H0 H1] H2] H3] H4] H5] OWN".
+    iPoseProof (black_white_update with "H3 OWN") as "> [H3 OWN]".
+    iModIntro. iFrame.
+  Qed.
+
+  Lemma default_I_update_ident_tgt ths im_src im_tgt0 st_src st_tgt im_tgt' im_tgt1
+    :
+    (default_I ths im_src im_tgt0 st_src st_tgt)
+      -∗
+      (OwnM (Auth.white (Excl.just im_tgt': @Excl.t (imap ident_tgt nat_wf)): identTgtRA))
+      -∗
+      #=> (OwnM (Auth.white (Excl.just im_tgt1: @Excl.t (imap ident_tgt nat_wf))) ** default_I ths im_src (imap_sum_id (fst (imap_proj_id im_tgt0), im_tgt1)) st_src st_tgt).
+  Proof.
+    unfold default_I. iIntros "[[[[[H0 H1] H2] H3] H4] H5] OWN".
+    iPoseProof (black_white_update with "H4 OWN") as "> [H4 OWN]".
+    ss. iModIntro. iFrame.
+  Qed.
+
+  Lemma default_I_update_ident_ths ths im_src im_tgt0 st_src st_tgt im_tgt' im_tgt1
+    :
+    (default_I ths im_src im_tgt0 st_src st_tgt)
+      -∗
+      (OwnM (Auth.white (Excl.just im_tgt': @Excl.t (imap thread_id nat_wf)): identThsRA))
+      -∗
+      #=> (OwnM (Auth.white (Excl.just im_tgt1: @Excl.t (imap thread_id nat_wf))) ** default_I ths im_src (imap_sum_id (im_tgt1, snd (imap_proj_id im_tgt0))) st_src st_tgt).
+  Proof.
+    unfold default_I. iIntros "[[[[[H0 H1] H2] H3] H4] H5] OWN".
+    iPoseProof (black_white_update with "H5 OWN") as "> [H5 OWN]".
+    ss. iModIntro. iFrame.
+  Qed.
+
+  Lemma default_I_get_st_src ths im_src im_tgt st_src st_tgt st_src'
+    :
+    (default_I ths im_src im_tgt st_src st_tgt)
+      -∗
+      (OwnM (Auth.white (Excl.just st_src': @Excl.t state_src): stateSrcRA))
+      -∗
+      ⌜st_src = st_src'⌝.
+  Proof.
+    unfold default_I. iIntros "[[[[[H0 H1] H2] H3] H4] H5] OWN".
+    iApply (black_white_equal with "H1 OWN").
+  Qed.
+
+  Lemma default_I_get_st_tgt ths im_src im_tgt st_src st_tgt st_tgt'
+    :
+    (default_I ths im_src im_tgt st_src st_tgt)
+      -∗
+      (OwnM (Auth.white (Excl.just st_tgt': @Excl.t state_tgt): stateTgtRA))
+      -∗
+      ⌜st_tgt = st_tgt'⌝.
+  Proof.
+    unfold default_I. iIntros "[[[[[H0 H1] H2] H3] H4] H5] OWN".
+    iApply (black_white_equal with "H2 OWN").
+  Qed.
+
+  Lemma default_I_get_ident_src ths im_src im_tgt st_src st_tgt im_src'
+    :
+    (default_I ths im_src im_tgt st_src st_tgt)
+      -∗
+      (OwnM (Auth.white (Excl.just im_src': @Excl.t (imap ident_src wf_src)): identSrcRA))
+      -∗
+      ⌜im_src = im_src'⌝.
+  Proof.
+    unfold default_I. iIntros "[[[[[H0 H1] H2] H3] H4] H5] OWN".
+    iApply (black_white_equal with "H3 OWN").
+  Qed.
+
+  Lemma default_I_get_ident_tgt ths im_src im_tgt st_src st_tgt im_tgt'
+    :
+    (default_I ths im_src im_tgt st_src st_tgt)
+      -∗
+      (OwnM (Auth.white (Excl.just im_tgt': @Excl.t (imap ident_tgt nat_wf)): identTgtRA))
+      -∗
+      ⌜snd (imap_proj_id im_tgt) = im_tgt'⌝.
+  Proof.
+    unfold default_I. iIntros "[[[[[H0 H1] H2] H3] H4] H5] OWN".
+    iApply (black_white_equal with "H4 OWN").
+  Qed.
+
+  Lemma default_I_get_ident_ths ths im_src im_tgt st_src st_tgt im_tgt'
+    :
+    (default_I ths im_src im_tgt st_src st_tgt)
+      -∗
+      (OwnM (Auth.white (Excl.just im_tgt': @Excl.t (imap thread_id nat_wf)): identThsRA))
+      -∗
+      ⌜fst (imap_proj_id im_tgt) = im_tgt'⌝.
+  Proof.
+    unfold default_I. iIntros "[[[[[H0 H1] H2] H3] H4] H5] OWN".
+    iApply (black_white_equal with "H5 OWN").
+  Qed.
+
+  Lemma default_I_thread_alloc ths0 im_src im_tgt st_src st_tgt ths'
+        tid ths1
+        (THS: TIdSet.add_new tid ths0 ths1)
+    :
+    (default_I ths' im_src im_tgt st_src st_tgt)
+      -∗
+      (own_threads_white ths0)
+      -∗
+      #=> (own_thread tid ** own_threads_white ths1 ** default_I ths1 im_src im_tgt st_src st_tgt).
+  Proof.
+    unfold default_I. iIntros "[[[[[H0 H1] H2] H3] H4] H5] H6".
+    iPoseProof (threads_alloc with "H0 H6") as "> [[BLACK WHITE] TH]".
+    { eauto. }
+    iModIntro. iFrame.
+  Qed.
+
+  Lemma default_I_thread_dealloc ths0 im_src im_tgt st_src st_tgt ths'
+        tid
+    :
+    (default_I ths' im_src im_tgt st_src st_tgt)
+      -∗
+      (own_threads_white ths0)
+      -∗
+      (own_thread tid)
+      -∗
+      ∃ ths1, ⌜NatMap.remove tid ths0 = ths1⌝ ** #=> (own_threads_white ths1 ** default_I ths1 im_src im_tgt st_src st_tgt).
+  Proof.
+    unfold default_I. iIntros "[[[[[H0 H1] H2] H3] H4] H5] THS TH".
+    iPoseProof (threads_dealloc with "H0 THS TH") as (ths1) "[% H0]".
+    iExists _. iSplit; eauto. iMod "H0". iModIntro.
+    iDestruct "H0" as "[H0 H6]". iFrame.
+  Qed.
+
+  Lemma default_I_ths_eq ths im_src im_tgt st_src st_tgt ths'
+    :
+    (default_I ths im_src im_tgt st_src st_tgt)
+      -∗
+      (own_threads_white ths')
+      -∗
+      ⌜ths = ths'⌝.
+  Proof.
+    unfold default_I. iIntros "[[[[[H0 H1] H2] H3] H4] H5] THS".
+    iApply (threads_eq with "H0 THS").
+  Qed.
+
 End INVARIANT.
