src/ThreadsRA.v
@@ -10,13 +10,17 @@ Set Implicit Arguments.
 Section THREADS_RA_DEF.
   Definition ths_RA: URA.t. Admitted.
 
-  Definition ths_RA_set (ths: TIdSet.t): ths_RA.(URA.car). Admitted.
+  Definition ths_RA_black (ths: TIdSet.t): ths_RA.(URA.car). Admitted.
+
+  Definition ths_RA_white (ths: TIdSet.t): ths_RA.(URA.car). Admitted.
 
   Definition ths_RA_th (th: thread_id): ths_RA.(URA.car). Admitted.
 
   Context `{@GRA.inG ths_RA Σ}.
 
-  Definition own_threads (ths: TIdSet.t): iProp := OwnM (ths_RA_set ths).
+  Definition own_threads_black (ths: TIdSet.t): iProp := OwnM (ths_RA_black ths).
+
+  Definition own_threads_white (ths: TIdSet.t): iProp := OwnM (ths_RA_white ths).
 
   Definition own_thread (th: thread_id): iProp := OwnM (ths_RA_th th).
 
@@ -25,18 +29,24 @@ Section THREADS_RA_DEF.
     (own_thread th0) -∗ (own_thread th1) -∗ ⌜th0 <> th1⌝.
   Admitted.
 
-  Lemma threads_alloc tid ths0 ths1
+  Lemma threads_eq ths ths'
     :
-    own_threads ths0 -∗ ⌜TIdSet.add_new tid ths0 ths1⌝ -∗ (own_threads ths1 ** own_thread tid).
+    (own_threads_black ths) -∗ (own_threads_white ths') -∗ ⌜ths = ths'⌝.
   Admitted.
 
-  Lemma threads_dealloc tid ths0
+  Lemma threads_alloc tid ths0 ths1 ths'
+        (THS: TIdSet.add_new tid ths0 ths1)
     :
-    own_threads ths0 -∗ own_thread tid -∗ ∃ ths1, ⌜NatMap.remove tid ths0 = ths1⌝ ** own_threads ths1.
+    own_threads_black ths' -∗ own_threads_white ths0 -∗ #=> (own_threads_black ths1 **own_threads_white ths1 ** own_thread tid).
+  Admitted.
+
+  Lemma threads_dealloc tid ths0 ths'
+    :
+    own_threads_black ths' -∗ own_threads_white ths0 -∗ own_thread tid -∗ ∃ ths1, ⌜NatMap.remove tid ths0 = ths1⌝ ** #=> (own_threads_black ths1 ** own_threads_white ths1).
   Admitted.
 
   Lemma threads_in tid ths
     :
-    own_threads ths -∗ own_thread tid -∗ ⌜TIdSet.In tid ths⌝.
+    own_threads_white ths -∗ own_thread tid -∗ ⌜TIdSet.In tid ths⌝.
   Admitted.
 End THREADS_RA_DEF.
